\begin{figure}
\begin{center}
\cfgstart
\cfgrule{$\phi$}{($\phi$) 
\cfgor $\phi \bowtie \phi$ 
\cfgor $\neg\phi$
\cfgor \cfgt{true}
\cfgor \cfgt{false}
\cfgor \cfgnt{r} $=$ \cfgnt{r}
\cfgor \cfgnt{r} $\neq$ \cfgnt{r}}
\cfgrule{l}{\cfgt{number}}
\cfgrule{\cfgnt{L}}{(\cfgnt{mt}
\cfgor (\cfgnt{L}\ [\cfgnt{r} $\rightarrow$ \{($\phi$\ \cfgnt{l})\ ...\}]))}
\cfgrule{\cfgnt{R}}{(\cfgnt{mt}
\cfgor (\cfgnt{R}\ [(\cfgnt{l}\ \cfgnt{f}) $\rightarrow$ \cfgnt{r}]))}
\cfgrule{$\eta$}{(\cfgnt{mt}
\cfgor ($\eta$\ [\cfgnt{x} $\rightarrow$ \cfgnt{v}]))}
\cfgrule{s}{\lp$\mu$ \cfgnt{L} \cfgnt{R} $\phi_g$ $\eta$ \cfgnt{e} \cfgnt{k}\rp}
\cfgrule{k}{\cfgt{end}
\cfgor{\lp \cfgt{*} \cfgt{\$} \cfgnt{f} $\rightarrow$ \cfgnt{k}\rp}
\cfgor{\lp \cfgnt{x} \cfgt{\$} \cfgnt{f}  \cfgt{:=} \cfgnt{*} $\rightarrow$ \cfgnt{k}\rp}}
\cfgorline{\lp \cfgt{*} \cfgt{=} \cfgnt{e} $\rightarrow$ \cfgnt{k}\rp
\cfgor{\lp \cfgnt{v} \cfgt{=} \cfgnt{*} $\rightarrow$ \cfgnt{k}\rp}
\cfgor{\lp \cfgt{if} \cfgnt{*} \cfgnt{e} \cfgt{else} \cfgnt{e} $\rightarrow$ \cfgnt{k} \rp}}
\cfgorline{\lp\cfgt{var} \cfgnt{T} \cfgnt{x} \cfgt{:=} \cfgnt{*} \cfgt{in} \cfgnt{e}  $\rightarrow$ \cfgnt{k} \rp
\cfgor{\lp \cfgnt{x} \cfgt{:=} \cfgnt{*} $\rightarrow$ \cfgnt{k}\rp}}
\cfgorline{\lp \cfgt{*} \cfgt{@} \cfgnt{m} \cfgnt{e} $\rightarrow$ \cfgnt{k} \rp
\cfgor{\lp \cfgnt{v} \cfgt{@} \cfgnt{m} \cfgt{*} $\rightarrow$ \cfgnt{k} \rp}}
\cfgorline{\lp\cfgt{begin}  \cfgnt{*} \lp \cfgnt{e} ...\rp $\rightarrow$ \cfgnt{k} \rp
\cfgor{\lp\cfgt{pop} $\eta$ \cfgnt{k}\rp}}
\cfgend
\end{center}
\caption{The machine syntax with $\bowtie \in \{\wedge,\vee,\Rightarrow\}$.}
\label{fig:machine-syntax}
\end{figure}
